realloc optimizations
- when old and new allocations would be large,
if new_size <= old_size, do not realloc,
return the original pointer
- when old and new allocations would be small,
if they would belong to the same sizeclass, do not realloc,
return the original pointer

dist/StarMalloc.c
@@ -2215,10 +2215,11 @@ static bool slab_free(uint8_t *ptr)
     return false;
 }
 
+size_t StarMalloc_threshold = (size_t)4096U - (size_t)2U;
+
 uint8_t *StarMalloc_malloc(size_t arena_id, size_t size)
 {
-  size_t threshold = (size_t)4096U - (size_t)2U;
-  if (size <= threshold)
+  if (size <= StarMalloc_threshold)
   {
     uint8_t *ptr = slab_malloc(arena_id, (uint32_t)size);
     if (ptr == NULL || false)
@@ -2249,13 +2250,11 @@ uint8_t *StarMalloc_malloc(size_t arena_id, size_t size)
 
 uint8_t *StarMalloc_aligned_alloc(size_t arena_id, size_t alignment, size_t size)
 {
-  size_t page_as_sz = (size_t)4096U;
   bool check = alignment > (size_t)0U && (size_t)4096U % alignment == (size_t)0U;
   if (check)
   {
     uint32_t alignment_as_u32 = (uint32_t)alignment;
-    size_t threshold = page_as_sz - (size_t)2U;
-    if (size <= threshold)
+    if (size <= StarMalloc_threshold)
     {
       uint8_t *ptr = slab_aligned_alloc(arena_id, alignment_as_u32, (uint32_t)size);
       if (ptr == NULL || false)
@@ -2345,9 +2344,24 @@ uint8_t *StarMalloc_realloc(size_t arena_id, uint8_t *ptr, size_t new_size)
   {
     size_t old_size = StarMalloc_getsize(ptr);
     bool old_allocation_is_small = old_size <= (size_t)4096U;
+    bool new_allocation_is_small = new_size <= StarMalloc_threshold;
+    bool same_case = old_allocation_is_small == new_allocation_is_small;
+    bool small_case_optim_condition;
+    if (old_allocation_is_small && same_case)
+    {
+      uint32_t r0 = SizeClassSelection_inv_impl((uint32_t)old_size);
+      size_t old_sc = (size_t)r0;
+      uint32_t r = SizeClassSelection_inv_impl((uint32_t)(new_size + (size_t)2U));
+      size_t new_sc = (size_t)r;
+      small_case_optim_condition = old_sc == new_sc;
+    }
+    else
+      small_case_optim_condition = false;
+    bool
+    large_case_optim_condition = !old_allocation_is_small && same_case && new_size <= old_size;
     if (old_size == (size_t)0U)
       return NULL;
-    else if (new_size <= old_size && !old_allocation_is_small)
+    else if (small_case_optim_condition || large_case_optim_condition)
       return ptr;
     else
     {
